wip

theories/Hoare.v
@@ -5,6 +5,7 @@ Local Open Scope string_scope.
 Local Open Scope Z_scope.
 Local Open Scope com_scope.
 
+Ltac inv H := inversion H; clear H; subst.
 
 Definition swap_xy :=
     ASSIGN "t" (VAR "x");; ASSIGN "x" (VAR "y");; ASSIGN "y" (VAR "t").
@@ -84,6 +85,12 @@ Notation "P -->> Q" := (aimp P Q) (at level 95, no associativity).
 Notation "P //\\ Q" := (aand P Q) (at level 80, right associativity).
 Notation "P \\// Q" := (aor P Q) (at level 75, right associativity).
 
+Ltac Tauto :=
+  let s := fresh "s" in
+  unfold aand, aor, aimp in *;
+  intro s;
+  repeat (match goal with [ H: (forall (s': store), _) |- _ ] => specialize (H s) end);
+  intuition auto.
 
 (** The rules of weak Hoare logic *)
 
@@ -97,95 +104,63 @@ Notation "P \\// Q" := (aor P Q) (at level 75, right associativity).
   of the command [c].  What is guaranteed is that if [c] terminates,
   then its final store satisfies postcondition [Q]. *)
 
-Inductive Hoare: assertion -> com -> assertion -> Prop :=
-| Hoare_skip: forall P,
-  (* ------------------ *)
-  Hoare P SKIP P
-| Hoare_assign: forall P x a,
-  (* ------------------------------ *)
-    Hoare (aupdate x a P) (ASSIGN x a) P
-| Hoare_seq: forall P Q R c1 c2,
-    Hoare P c1 Q ->
-    Hoare Q c2 R ->
-    (* ------------------ *)
-    Hoare P (c1 ;; c2) R
-| Hoare_choice: forall P Q c1 c2,
-    Hoare P c1 Q ->
-    Hoare P c2 Q ->
-    (* ---------------------- *)
-    Hoare P (c1 ⊕ c2) Q
-| Hoare_consequence: forall P Q P' Q' c,
-    Hoare P c Q ->
-    P' -->> P ->
-    Q -->> Q' ->
-    (* -------------*)
-    Hoare P' c Q'
-| Hoare_cstar: forall INV c, 
-    Hoare INV c INV ->
-    (* ------------------ *)
-    Hoare INV (CSTAR c) INV.
+Reserved Notation "⦃ P ⦄ c ⦃ Q ⦄" (at level 90, c at next level).
 
-Reserved Notation "'hoare' p '<<' c '>>' q"
-  (at level 40, p at level 39, c at level 99, q at level 39).
-
-Inductive HoareRes: assertion -> com -> postassertion -> Prop :=
+Inductive WeakHoareRes: assertion -> com -> postassertion -> Prop :=
 | Hoare_skip_r: forall P,
   (* ------------------ *)
-  hoare P << SKIP >> P
+  ⦃ P ⦄ SKIP ⦃ P ⦄
 | Hoare_assign_r: forall P x a,
   (* ------------------------------ *)
-    hoare (aupdate x a P) << ASSIGN x a >> P
+    ⦃ aupdate x a P ⦄ ASSIGN x a ⦃ P ⦄
 | Hoare_seq_ok: forall P Q R c1 c2,
-    hoare P << c1 >> Q ->
-    hoare Q << c2 >> R ->
+    ⦃ P ⦄ c1 ⦃ Q ⦄ ->
+    ⦃ Q ⦄ c2 ⦃ R ⦄ ->
     (* ------------------ *)
-    hoare P << (c1 ;; c2) >> R
+    ⦃ P ⦄ (c1 ;; c2) ⦃ R ⦄
 | Hoare_seq_err: forall P c1 c2,
-    HoareRes P c1 (fun r => match r with RError => True | _ => False end) ->
+    WeakHoareRes P c1 (fun r => match r with RError _ => True | _ => False end) ->
     (* ------------------ *)
-    HoareRes P (c1 ;; c2) (fun r => match r with RError => True | _ => False end)
+    WeakHoareRes P (c1 ;; c2) (fun r => match r with RError _ => True | _ => False end)
 | Hoare_consequence_res: forall P Q P' Q' c,
-    hoare P << c >> Q ->
+    ⦃ P ⦄ c ⦃ Q ⦄ ->
     P' -->> P ->
     Q -->> Q' ->
     (* -------------*)
-    hoare P' << c >> Q'
+    ⦃ P' ⦄ c ⦃ Q' ⦄
 | Hoare_choice_res: forall P Q c1 c2,
-    hoare P << c1 >> Q ->
-    hoare P << c2 >> Q ->
+    ⦃ P ⦄ c1 ⦃ Q ⦄ ->
+    ⦃ P ⦄ c2 ⦃ Q ⦄ ->
     (* ---------------------- *)
-    hoare P << c1 ⊕ c2 >> Q
+    ⦃ P ⦄ (c1 ⊕ c2) ⦃ Q ⦄
 | Hoare_cstar_ress: forall INV c, 
-    hoare INV << c >> INV ->
+    ⦃ INV ⦄ c ⦃ INV ⦄ ->
     (* ------------------ *)
-    hoare INV << CSTAR c >> INV
-where "'hoare' p '<<' c '>>' q" :=
-  (HoareRes p c (fun r => match r with
-                          | RNormal s => q s
-                          | RError => False
+    ⦃ INV ⦄ (CSTAR c) ⦃ INV ⦄
+where "⦃ P ⦄ c ⦃ Q ⦄" :=
+  (WeakHoareRes P c (fun r => match r with
+                          | RNormal s => Q s
+                          | RError _ => False
                           end)).
 
-
 Lemma Hoare_consequence_pre: forall P P' Q c,
-      hoare P << c >> Q ->
+      ⦃ P ⦄ c ⦃ Q ⦄ ->
       P' -->> P ->
-      hoare P' << c >> Q.
+      ⦃ P' ⦄ c ⦃ Q ⦄.
 Proof.
   intros. apply Hoare_consequence_res with (P := P) (Q := Q); unfold aimp; auto.
 Qed.
 
 Lemma Hoare_consequence_post: forall P Q Q' c,
-      hoare P << c >> Q ->
+      ⦃ P ⦄ c ⦃ Q ⦄ ->
       Q -->> Q' ->
-      hoare P << c >> Q'.
+      ⦃ P ⦄ c ⦃ Q' ⦄.
 Proof.
   intros. apply Hoare_consequence_res with (P := P) (Q := Q); unfold aimp; auto.
 Qed.
 
 Example Hoare_swap_xy: forall m n,
-  hoare (aequal (VAR "x") m //\\ aequal (VAR "y") n)
-        << swap_xy >>
-        (aequal (VAR "x") n //\\ aequal (VAR "y") m).
+  ⦃ (aequal (VAR "x") m //\\ aequal (VAR "y") n) ⦄ swap_xy ⦃ (aequal (VAR "x") n //\\ aequal (VAR "y") m) ⦄.
 Proof.
   intros.
   eapply Hoare_consequence_pre.
@@ -204,17 +179,17 @@ Qed.
 Definition triple (P: assertion) (c: com) (Q: assertion) : Prop :=
   forall s r, cexec s c r -> P s -> (exists s', r = RNormal s' /\ Q s').
 
-Notation "{{ P }} c {{ Q }}" := (triple P c Q) (at level 90, c at next level).
+Notation "⦃⦃ P ⦄⦄ c ⦃⦃ Q ⦄⦄" := (triple P c Q) (at level 90, c at next level).
 
 Lemma triple_skip: forall P,
-     {{P}} SKIP {{P}}.
+     ⦃⦃ P ⦄⦄ SKIP ⦃⦃ P ⦄⦄.
 Proof.
   unfold triple; intros. exists s. inversion H; subst. auto.
 Qed.
 
 
 Lemma triple_assign: forall P x a,
-      {{aupdate x a P}} ASSIGN x a {{P}}.
+      ⦃⦃ aupdate x a P ⦄⦄ ASSIGN x a ⦃⦃ P ⦄⦄.
 Proof.
   unfold triple, aupdate; intros P x a s r EXEC PRE.
   inversion EXEC; subst.
@@ -222,9 +197,9 @@ Proof.
 Qed.
 
 Lemma triple_seq: forall P Q R c1 c2,
-      {{P}} c1 {{Q}} ->
-      {{Q}} c2 {{R}} ->
-      {{P}} c1;;c2 {{R}}.
+      ⦃⦃ P ⦄⦄ c1 ⦃⦃ Q ⦄⦄ ->
+      ⦃⦃ Q ⦄⦄ c2 ⦃⦃ R ⦄⦄ ->
+      ⦃⦃ P ⦄⦄ c1;;c2 ⦃⦃ R ⦄⦄.
 Proof.
   unfold triple; intros P Q R c1 c2 H1 H2 s r EXEC PRE.
   inversion EXEC; subst.
@@ -240,23 +215,23 @@ Proof.
     end.
   - (* cexec_seq_error: c1 errors *)
     match goal with
-    | E1 : cexec s c1 RError |- _ =>
-      destruct (H1 s RError E1 PRE) as (? & EQ & _); discriminate
+    | E1 : cexec s c1 (RError ?se) |- _ =>
+      destruct (H1 s (RError se) E1 PRE) as (? & EQ & _); discriminate
     end.
   - (* cexec_seq_error_right: c1 normal, c2 errors *)
     match goal with
     | E1 : cexec s c1 (RNormal ?s'),
-      E2 : cexec ?s' c2 RError |- _ =>
+      E2 : cexec ?s' c2 (RError ?se) |- _ =>
       destruct (H1 s (RNormal s') E1 PRE) as (sx & EQ1 & QSx);
       inversion EQ1; subst sx;
-      destruct (H2 s' RError E2 QSx) as (? & EQ & _); discriminate
+      destruct (H2 s' (RError se) E2 QSx) as (? & EQ & _); discriminate
     end.
 Qed.
 
 Lemma triple_ifthenelse: forall P Q b c1 c2,
-      {{atrue b //\\ P}} c1 {{Q}} ->
-      {{afalse b //\\ P}} c2 {{Q}} ->
-      {{P}} IF b THEN c1 ELSE c2 END {{Q}}.
+      ⦃⦃ atrue b //\\ P ⦄⦄ c1 ⦃⦃ Q ⦄⦄ ->
+      ⦃⦃ afalse b //\\ P ⦄⦄ c2 ⦃⦃ Q ⦄⦄ ->
+      ⦃⦃ P ⦄⦄ IF b THEN c1 ELSE c2 END ⦃⦃ Q ⦄⦄.
 Proof.
   unfold triple, aand, atrue, afalse.
   intros P Q b c1 c2 H1 H2 s r EXEC PRE.
@@ -267,7 +242,7 @@ Proof.
       match goal with EA : cexec s (ASSUME b) _ |- _ => inversion EA; subst end.
       eapply H1; eauto.
     + (* SEQ error left: ASSUME b errors — impossible *)
-      match goal with EA : cexec s (ASSUME b) RError |- _ => inversion EA end.
+      match goal with EA : cexec s (ASSUME b) (RError _) |- _ => inversion EA end.
     + (* SEQ error right *)
       match goal with EA : cexec s (ASSUME b) _ |- _ => inversion EA; subst end.
       eapply H1; eauto.
@@ -276,7 +251,7 @@ Proof.
     + match goal with EA : cexec s (ASSUME (NOT b)) _ |- _ => inversion EA; subst end.
       eapply H2; eauto.
       split; [ apply Bool.negb_true_iff; assumption | exact PRE ].
-    + match goal with EA : cexec s (ASSUME (NOT b)) RError |- _ => inversion EA end.
+    + match goal with EA : cexec s (ASSUME (NOT b)) (RError _) |- _ => inversion EA end.
     + match goal with EA : cexec s (ASSUME (NOT b)) _ |- _ => inversion EA; subst end.
       eapply H2; eauto.
       split; [ apply Bool.negb_true_iff; assumption | exact PRE ].
@@ -285,7 +260,7 @@ Qed.
 (** Helper: [P] is preserved across any number of iterations of the loop body
     [(ASSUME b ;; c)] when [c] preserves [P] under the [b]-true precondition. *)
 Lemma triple_while_invariant: forall P b c s s',
-  {{atrue b //\\ P}} c {{P}} ->
+  ⦃⦃ atrue b //\\ P ⦄⦄ c ⦃⦃ P ⦄⦄ ->
   star (step_iter (ASSUME b ;; c)) s s' ->
   P s -> P s'.
 Proof.
@@ -310,19 +285,19 @@ Lemma cexec_seq_inv:
   forall c1 c2 s r,
     cexec s (c1 ;; c2) r ->
     (exists sm sf, cexec s c1 (RNormal sm) /\ cexec sm c2 (RNormal sf) /\ r = RNormal sf)
-    \/ (cexec s c1 RError /\ r = RError)
-    \/ (exists sm, cexec s c1 (RNormal sm) /\ cexec sm c2 RError /\ r = RError).
+    \/ (exists sf, cexec s c1 (RError sf) /\ r = RError sf)
+    \/ (exists sm sf, cexec s c1 (RNormal sm) /\ cexec sm c2 (RError sf) /\ r = RError sf).
 Proof.
   intros c1 c2 s r EXEC.
   inversion EXEC; subst.
   - left. eauto.
-  - right. left. auto.
+  - right. left. eauto.
   - right. right. eauto.
 Qed.
 
 Lemma triple_while: forall P b c,
-      {{atrue b //\\ P}} c {{P}} ->
-      {{P}} WHILE b DO c END {{afalse b //\\ P}}.
+      ⦃⦃ atrue b //\\ P ⦄⦄ c ⦃⦃ P ⦄⦄ ->
+      ⦃⦃ P ⦄⦄ WHILE b DO c END ⦃⦃ afalse b //\\ P ⦄⦄.
 Proof.
   unfold triple, aand, atrue, afalse.
   intros P b c H s r EXEC PRE.
@@ -330,7 +305,7 @@ Proof.
   apply cexec_seq_inv in EXEC.
   destruct EXEC as
     [ (sm & sf & EI & EA & ->)
-    | [ (EI & ->) | (sm & EI & EA & ->) ] ].
+    | [ (sf & EI & ->) | (sm & sf & EI & EA & ->) ] ].
   - (* SEQ normal *)
     apply cexec_cstar_iff_star in EI.
     assert (PSm : P sm) by (eapply triple_while_invariant; eauto).
@@ -346,24 +321,24 @@ Proof.
     apply cexec_seq_inv in ERR.
     destruct ERR as
       [ (sm1 & sf1 & _ & _ & EQbad)
-      | [ (EA & _) | (sx & EA & EC & _) ] ].
+      | [ (sf1 & EA & _) | (sx & sf1 & EA & EC & _) ] ].
     + (* normal yields RNormal, can't equal RError *)
       discriminate EQbad.
     + (* ASSUME b errors: impossible *)
       inversion EA.
     + (* ASSUME b ok, c errors: contradicts H. EA : cexec sm (ASSUME b) (RNormal sx) *)
-      inversion EA; subst sx.   (* substitute sx := sm only *)
-      destruct (H sm RError EC) as (? & EQc & _);
+      inversion EA; subst sx.
+      destruct (H sm (RError sf1) EC) as (? & EQc & _);
         [ split; assumption | discriminate ].
   - (* SEQ error right: ASSUME (NOT b) errors. Impossible. *)
     inversion EA.
 Qed.
 
 Lemma triple_consequence: forall P Q P' Q' c,
-      {{P}} c {{Q}} ->
+      ⦃⦃ P ⦄⦄ c ⦃⦃ Q ⦄⦄ ->
       P' -->> P ->
       Q -->> Q' ->
-      {{P'}} c {{Q'}}.
+      ⦃⦃ P' ⦄⦄ c ⦃⦃ Q' ⦄⦄.
 Proof.
   unfold triple, aimp; intros P Q P' Q' c HT P'P QQ' s r EXEC PRE.
   destruct (HT s r EXEC (P'P s PRE)) as (s' & EQ & QSx).
@@ -371,8 +346,187 @@ Proof.
 Qed.
 
 (** Strong Hoare triples *)
+Reserved Notation "⦇ P ⦈ c ⦇ Q ⦈" (at level 90, c at next level).
+
+Definition alessthan (a: aexp) (v: Z) : assertion :=
+  fun s => 0 <= aeval a s < v.
+
+Inductive StrongHoareRes: assertion -> com -> postassertion -> Prop :=
+| HOARE_skip_r: forall P,
+  (* ------------------ *)
+  ⦇ P ⦈ SKIP ⦇ P ⦈
+| HOARE_assign_r: forall P x a,
+  (* ------------------------------ *)
+    ⦇ aupdate x a P ⦈ ASSIGN x a ⦇ P ⦈
+| HOARE_seq_ok: forall P Q R c1 c2,
+    ⦇ P ⦈ c1 ⦇ Q ⦈ ->
+    ⦇ Q ⦈ c2 ⦇ R ⦈ ->
+    (* ------------------ *)
+    ⦇ P ⦈ (c1 ;; c2) ⦇ R ⦈
+| HOARE_seq_err: forall P c1 c2,
+    StrongHoareRes P c1 (fun r => match r with RError _ => True | _ => False end) ->
+    (* ------------------ *)
+    StrongHoareRes P (c1 ;; c2) (fun r => match r with RError _ => True | _ => False end)
+| HOARE_consequence_res: forall P Q P' Q' c,
+    ⦇ P ⦈ c ⦇ Q ⦈ ->
+    P' -->> P ->
+    Q -->> Q' ->
+    (* -------------*)
+    ⦇ P' ⦈ c ⦇ Q' ⦈
+| HOARE_choice_res: forall P Q c1 c2,
+    ⦇ P ⦈ c1 ⦇ Q ⦈ ->
+    ⦇ P ⦈ c2 ⦇ Q ⦈ ->
+    (* ---------------------- *)
+    ⦇ P ⦈ (c1 ⊕ c2) ⦇ Q ⦈
+| HOARE_cstar_ress: forall INV c a, 
+    (forall v,  ⦇ INV //\\ aequal a v ⦈ c ⦇ alessthan a v //\\ INV ⦈ ) ->
+    (* ------------------ *)
+    ⦇ INV ⦈ (CSTAR c) ⦇ INV ⦈
+where "⦇ P ⦈ c ⦇ Q ⦈" :=
+  (StrongHoareRes P c (fun r => match r with
+                          | RNormal s => Q s
+                          | RError _ => False
+                          end)).
+
 
 Definition Triple (P: assertion) (c: com) (Q: assertion) :=
   forall s, P s -> exists s', cexec s c (RNormal s') /\ Q s'.
 
-Notation "{{{ P }}} c {{{ Q }}}" := (Triple P c Q) (at level 90, c at next level).
+Notation "⦇⦇ P ⦈⦈ c ⦇⦇ Q ⦈⦈" := (Triple P c Q) (at level 90, c at next level).
+
+
+Lemma Triple_skip: forall P, 
+  ⦇⦇ P ⦈⦈ SKIP ⦇⦇ P ⦈⦈.
+Proof.
+  unfold Triple; intros. exists s. split; [ apply cexec_skip | exact H ].
+Qed.
+
+Lemma Triple_assign: forall P x a,
+      ⦇⦇ aupdate x a P ⦈⦈ ASSIGN x a ⦇⦇ P ⦈⦈.
+Proof.
+  unfold Triple, aupdate; intros P x a s PRE.
+  exists (update x (aeval a s) s). split; [ apply cexec_assign | exact PRE ].
+Qed.
+
+Lemma Triple_seq: forall P Q R c1 c2,
+      ⦇⦇ P ⦈⦈ c1 ⦇⦇ Q ⦈⦈ -> ⦇⦇ Q ⦈⦈ c2 ⦇⦇ R ⦈⦈ ->
+      ⦇⦇ P ⦈⦈ c1;;c2 ⦇⦇ R ⦈⦈.
+Proof.
+  unfold Triple; intros P Q R c1 c2 H1 H2 s PRE.
+  destruct (H1 s PRE) as (sm & EXEC1 & QSx).
+  destruct (H2 sm QSx) as (sf & EXEC2 & RSf).
+  exists sf. split; [ apply cexec_seq with sm; assumption | exact RSf ].
+Qed.
+
+Lemma Triple_ifthenelse: forall P Q b c1 c2,
+      ⦇⦇ atrue b //\\ P ⦈⦈ c1 ⦇⦇ Q ⦈⦈ ->
+      ⦇⦇ afalse b //\\ P ⦈⦈ c2 ⦇⦇ Q ⦈⦈ ->
+      ⦇⦇ P ⦈⦈ IF b THEN c1 ELSE c2 END ⦇⦇ Q ⦈⦈.
+Proof.
+  unfold Triple, aand, atrue, afalse; intros P Q b c1 c2 H1 H2 s PRE.
+  destruct (beval b s) eqn:Hb.
+  - destruct (H1 s (conj Hb PRE)) as (s' & EXEC & QS').
+    exists s'. split; [ | exact QS' ].
+    apply cexec_choice_left.
+    apply cexec_seq with s; [ apply cexec_assume; exact Hb | exact EXEC ].
+  - destruct (H2 s (conj Hb PRE)) as (s' & EXEC & QS').
+    exists s'. split; [ | exact QS' ].
+    apply cexec_choice_right.
+    apply cexec_seq with s;
+      [ apply cexec_assume; cbn; rewrite Hb; reflexivity | exact EXEC ].
+Qed.
+
+Lemma Triple_consequence: forall P Q P' Q' c,
+      ⦇⦇ P ⦈⦈ c ⦇⦇ Q ⦈⦈ ->
+      P' -->> P ->
+      Q -->> Q' ->
+      ⦇⦇ P' ⦈⦈ c ⦇⦇ Q' ⦈⦈.
+Proof.
+  unfold Triple, aimp; intros P Q P' Q' c HT HP'P HQQ' s PRE.
+  destruct (HT s (HP'P s PRE)) as (s' & EXEC & QS').
+  exists s'. split; [ exact EXEC | apply HQQ', QS' ].
+Qed.
+
+
+Lemma Triple_while: forall P variant b c,
+  (forall v,
+     ⦇⦇ P //\\ atrue b //\\ aequal variant v ⦈⦈
+     c
+     ⦇⦇ P //\\ alessthan variant v ⦈⦈)
+  ->
+     ⦇⦇ P ⦈⦈ WHILE b DO c END ⦇⦇ P //\\ afalse b ⦈⦈.
+Proof.
+  unfold Triple, aand, atrue, afalse, aequal, alessthan.
+  intros P variant b c H s0 PRE0.
+  (* Helper: from any P-state with non-negative variant, the iterated body
+     [(ASSUME b ;; c) ★] terminates in a state where [P] still holds and [b]
+     is false.  Proved by induction on a nat upper bound for [Z.to_nat] of
+     the variant. *)
+  assert (HELP: forall n s,
+              0 <= aeval variant s ->
+              (Z.to_nat (aeval variant s) <= n)%nat ->
+              P s ->
+              exists sf,
+                cexec s (CSTAR (ASSUME b ;; c)) (RNormal sf) /\
+                P sf /\ beval b sf = false).
+  { induction n as [|n IH]; intros s Hvnn Hn PS.
+    - (* n = 0: with 0 <= variant and Z.to_nat variant <= 0 we get variant = 0 *)
+      assert (Hzero : aeval variant s = 0).
+      { destruct (aeval variant s) as [|p|p]; lia. }
+      destruct (beval b s) eqn:Hb.
+      + (* b = true: H with v=0 demands [0 <= variant s1 < 0], contradiction *)
+        destruct (H 0 s) as (s1 & _ & _ & (Hv0 & Hlt)).
+        { split; [ exact PS | split; [ exact Hb | exact Hzero ] ]. }
+        lia.
+      + exists s. split; [ apply cexec_cstar_done | split; assumption ].
+    - destruct (beval b s) eqn:Hb.
+      + destruct (H (aeval variant s) s) as (s1 & EXEC1 & PS1 & (Hv0 & Hlt)).
+        { split; [ exact PS | split; [ exact Hb | reflexivity ] ]. }
+        assert (Hsmaller : (Z.to_nat (aeval variant s1) <= n)%nat).
+        { assert ((Z.to_nat (aeval variant s1) < Z.to_nat (aeval variant s))%nat)
+            by (apply (proj1 (Z2Nat.inj_lt _ _ Hv0 Hvnn)); exact Hlt).
+          lia. }
+        destruct (IH s1 Hv0 Hsmaller PS1) as (s2 & EXEC2 & PS2 & Hb2).
+        exists s2. split; [ | split; assumption ].
+        eapply cexec_cstar_step_ok.
+        * apply cexec_seq with s; [ apply cexec_assume; exact Hb | exact EXEC1 ].
+        * exact EXEC2.
+      + exists s. split; [ apply cexec_cstar_done | split; assumption ].
+  }
+  (* Main argument: case-split on initial b. The b-true case takes one
+     iteration first so that the variant becomes non-negative before HELP. *)
+  destruct (beval b s0) eqn:Hb.
+  - destruct (H (aeval variant s0) s0) as (s1 & EXEC1 & PS1 & (Hv0 & _)).
+    { split; [ exact PRE0 | split; [ exact Hb | reflexivity ] ]. }
+    destruct (HELP (Z.to_nat (aeval variant s1)) s1 Hv0 (le_n _) PS1)
+      as (sf & EXEC_LOOP & PSf & Hbf).
+    exists sf. split.
+    + apply cexec_seq with sf.
+      * eapply cexec_cstar_step_ok.
+        -- apply cexec_seq with s0;
+             [ apply cexec_assume; exact Hb | exact EXEC1 ].
+        -- exact EXEC_LOOP.
+      * apply cexec_assume; cbn; rewrite Hbf; reflexivity.
+    + split; [ exact PSf | exact Hbf ].
+  - exists s0. split.
+    + apply cexec_seq with s0.
+      * apply cexec_cstar_done.
+      * apply cexec_assume; cbn; rewrite Hb; reflexivity.
+    + split; [ exact PRE0 | exact Hb ].
+Qed.
+
+Module Soundness.
+  (* TODO *) 
+End Soundness.
+
+Module Completness.
+  (* TODO *) 
+End Completness.
+
+Module WP.
+  (* TODO *) 
+End WP.
+
+Module SP.
+  (* TODO *) 
+End SP.
