theories/Inc.v
@@ -1,0 +1,20 @@
+From Stdlib Require Import Arith ZArith Psatz Bool String List Program.Equality.
+From IncLogic Require Import Imp Sequences Hoare.
+
+Local Open Scope string_scope.
+Local Open Scope Z_scope.
+
+Reserved Notation "⟦ P ⟧ c ⟦ Q ⟧" (at level 90, c at next level).
+
+(* Notation "⟦ P ⟧ c ⟦ Q1 ⟧ ⟦ Q2 ⟧" := (⟦ P ⟧ c ⟦ Q1 ⟧ /\ ⟦ P ⟧ c ⟦ Q2 ⟧) (at level 90, c at next level). *)
+
+Definition afalse_assn : assertion := fun _ => False.
+
+
+Inductive Inc_triple: assertion -> com -> postassertion -> Prop :=
+| Inc_triple_skip: forall P,
+    ⟦ P ⟧ SKIP ⟦ P ⟧
+where "⟦ P ⟧ c ⟦ Q ⟧" := (Inc_triple P c (fun r => match r with
+    | RNormal s => Q s
+    | RError => False
+    end)).
